Test.lean
@@ -1,0 +1,19 @@
+/-! # how to test
+
+1. first, run `lake exe mdgen Test/Src Test/Out`
+2. run `lake exe test`
+-/
+
+def main : IO UInt32 := do
+  let firstActual ← IO.FS.readFile ⟨"Test/Out/first.md"⟩
+  let firstExpected ← IO.FS.readFile ⟨"Test/Exp/first.md"⟩
+  if firstActual != firstExpected then
+    IO.eprintln "first.md is not as expected"
+    return 1
+
+  let secondActual ← IO.FS.readFile ⟨"Test/Out/Second/second.md"⟩
+  let secondExpected ← IO.FS.readFile ⟨"Test/Exp/Second/second.md"⟩
+  if secondActual != secondExpected then
+    IO.eprintln "second.md is not as expected"
+    return 1
+  return 0
