Test/Src/First.lean
@@ -1,0 +1,13 @@
+/- # Propositional Logic -/
+
+variable (P Q : Prop)
+
+example (hQ : Q) : P → Q := by
+  intro _
+  exact hQ
+
+/-! this is a very easy exercise. -/
+
+example (h : P) : P ∨ Q := by
+  apply Or.inl
+  exact h
