Test/Src/Second/Second.lean
@@ -1,0 +1,7 @@
+/- # sample of doc comment and ignoring -/
+
+variable (n : Nat) --#
+
+/-- adding zero changes nothing -/
+theorem add_zero : n + 0 = n := by
+  rw [Nat.add_zero]
