lakefile.lean
@@ -16,3 +16,8 @@ lean_exe «mdgen» where
   -- executed when `lake exe mdgen` runs
   root := `Mdgen
   supportInterpreter := true
+
+lean_exe test where
+  -- executed when `lake exe test` runs
+  root := `Test
+  supportInterpreter := true
