Test/Exp/First.md
@@ -1,0 +1,17 @@
+# Propositional Logic
+
+```lean
+variable (P Q : Prop)
+
+example (hQ : Q) : P → Q := by
+  intro _
+  exact hQ
+```
+
+this is a very easy exercise.
+
+```lean
+example (h : P) : P ∨ Q := by
+  apply Or.inl
+  exact h
+```
