Test/Exp/Second/Second.md
@@ -1,0 +1,7 @@
+# sample of doc comment and ignoring
+
+```lean
+/-- adding zero changes nothing -/
+theorem add_zero : n + 0 = n := by
+  rw [Nat.add_zero]
+```
